ported fair Zip loop to new setup

Given_Clause_Loops/Fair_Zipperposition_Loop.thy
@@ -15,7 +15,7 @@ begin
 
 subsection \<open>Locale\<close>
 
-type_synonym ('t, 'p, 'f) fair_ZL_state = "'t \<times> 'p \<times> 'f option \<times> 'f fset"
+type_synonym ('t, 'p, 'f) fair_ZL_state = "'t \<times> 'f inference set \<times> 'p \<times> 'f option \<times> 'f fset"
 
 locale fair_zipperposition_loop =
   discount_loop Bot_F Inf_F Bot_G Q entails_q Inf_G_q Red_I_q Red_F_q \<G>_F_q \<G>_I_q Equiv_F Prec_F +
@@ -66,22 +66,24 @@ subsection \<open>Definition and Lemmas\<close>
 
 abbreviation todo_of :: "('t, 'p, 'f) fair_ZL_state \<Rightarrow> 't" where
   "todo_of St \<equiv> fst St"
+abbreviation done_of :: "('t, 'p, 'f) fair_ZL_state \<Rightarrow> 'f inference set" where
+  "done_of St \<equiv> fst (snd St)"
 abbreviation passive_of :: "('t, 'p, 'f) fair_ZL_state \<Rightarrow> 'p" where
-  "passive_of St \<equiv> fst (snd St)"
+  "passive_of St \<equiv> fst (snd (snd St))"
 abbreviation yy_of :: "('t, 'p, 'f) fair_ZL_state \<Rightarrow> 'f option" where
-  "yy_of St \<equiv> fst (snd (snd St))"
+  "yy_of St \<equiv> fst (snd (snd (snd St)))"
 abbreviation active_of :: "('t, 'p, 'f) fair_ZL_state \<Rightarrow> 'f fset" where
-  "active_of St \<equiv> snd (snd (snd St))"
+  "active_of St \<equiv> snd (snd (snd (snd St)))"
 
 abbreviation all_formulas_of :: "('t, 'p, 'f) fair_ZL_state \<Rightarrow> 'f set" where
   "all_formulas_of St \<equiv> passive.elems (passive_of St) \<union> set_option (yy_of St) \<union> fset (active_of St)"
 
 fun zl_fstate :: "('t, 'p, 'f) fair_ZL_state \<Rightarrow> 'f inference set \<times> ('f \<times> DL_label) set" where
-  "zl_fstate (T, P, Y, A) = zl_state (todo.elems T, passive.elems P, set_option Y, fset A)"
+  "zl_fstate (T, D, P, Y, A) = zl_state (todo.elems T, D, passive.elems P, set_option Y, fset A)"
 
 lemma zl_fstate_alt_def:
-  "zl_fstate St = zl_state (todo.elems (fst St), passive.elems (fst (snd St)),
-     set_option (fst (snd (snd St))), fset (snd (snd (snd St))))"
+  "zl_fstate St = zl_state (todo.elems (fst St), fst (snd St), passive.elems (fst (snd (snd St))),
+     set_option (fst (snd (snd (snd St)))), fset (snd (snd (snd (snd St)))))"
   by (cases St) auto
 
 definition
@@ -117,42 +119,45 @@ inductive
 where
   compute_infer: "T \<noteq> t_empty \<Longrightarrow> t_select T = LCons \<iota>0 \<iota>s \<Longrightarrow>
     \<iota>0 \<in> no_labels.Red_I (fset A \<union> {C}) \<Longrightarrow>
-    (T, P, None, A) \<leadsto>ZLf (t_add \<iota>s (t_remove (t_select T) T), p_add C P, None, A)"
+    (T, D, P, None, A) \<leadsto>ZLf (t_add \<iota>s (t_remove (t_select T) T), D \<union> {\<iota>0}, p_add C P, None, A)"
 | choose_p: "P \<noteq> p_empty \<Longrightarrow>
-    (T, P, None, A) \<leadsto>ZLf (T, p_remove (p_select P) P, Some (p_select P), A)"
+    (T, D, P, None, A) \<leadsto>ZLf (T, D, p_remove (p_select P) P, Some (p_select P), A)"
 | delete_fwd: "C \<in> no_labels.Red_F (fset A) \<or> (\<exists>C' \<in> fset A. C' \<preceq>\<cdot> C) \<Longrightarrow>
-    (T, P, Some C, A) \<leadsto>ZLf (T, P, None, A)"
+    (T, D, P, Some C, A) \<leadsto>ZLf (T, D, P, None, A)"
 | simplify_fwd: "C' \<prec>S C \<Longrightarrow> C \<in> no_labels.Red_F (fset A \<union> {C'}) \<Longrightarrow>
-    (T, P, Some C, A) \<leadsto>ZLf (T, P, Some C', A)"
+    (T, D, P, Some C, A) \<leadsto>ZLf (T, D, P, Some C', A)"
 | delete_bwd: "C' |\<notin>| A \<Longrightarrow> C' \<in> no_labels.Red_F {C} \<or> C' \<cdot>\<succ> C \<Longrightarrow>
-    (T, P, Some C, A |\<union>| {|C'|}) \<leadsto>ZLf (T, P, Some C, A)"
+    (T, D, P, Some C, A |\<union>| {|C'|}) \<leadsto>ZLf (T, D, P, Some C, A)"
 | simplify_bwd: "C' |\<notin>| A \<Longrightarrow> C'' \<prec>S C' \<Longrightarrow> C' \<in> no_labels.Red_F {C, C''} \<Longrightarrow>
-    (T, P, Some C, A |\<union>| {|C'|}) \<leadsto>ZLf (T, p_add C'' P, Some C, A)"
+    (T, D, P, Some C, A |\<union>| {|C'|}) \<leadsto>ZLf (T, D, p_add C'' P, Some C, A)"
 | schedule_infer: "flat_inferences_of (set \<iota>ss) = no_labels.Inf_between (fset A) {C} \<Longrightarrow>
-    (T, P, Some C, A) \<leadsto>ZLf (fold t_add \<iota>ss T, P, None, A |\<union>| {|C|})"
+    (T, D, P, Some C, A) \<leadsto>ZLf
+    (fold t_add \<iota>ss T, D - flat_inferences_of (set \<iota>ss), P, None, A |\<union>| {|C|})"
 | delete_orphan_infers: "\<iota>s \<in> todo.elems T \<Longrightarrow> lset \<iota>s \<inter> no_labels.Inf_from (fset A) = {} \<Longrightarrow>
-    (T, P, Y, A) \<leadsto>ZLf (t_remove \<iota>s T, P, Y, A)"
+    (T, D, P, Y, A) \<leadsto>ZLf (t_remove \<iota>s T, D, P, Y, A)"
 
 inductive
   compute_infer_step :: "('t, 'p, 'f) fair_ZL_state \<Rightarrow> ('t, 'p, 'f) fair_ZL_state \<Rightarrow> bool"
 where
   "T \<noteq> t_empty \<Longrightarrow> t_select T = LCons \<iota>0 \<iota>s \<Longrightarrow> \<iota>0 \<in> no_labels.Red_I (fset A \<union> {C}) \<Longrightarrow>
-   compute_infer_step (T, P, None, A) (t_add \<iota>s (t_remove (t_select T) T), p_add C P, None, A)"
+   compute_infer_step (T, D, P, None, A)
+     (t_add \<iota>s (t_remove (t_select T) T), D \<union> {\<iota>0}, p_add C P, None, A)"
 
 inductive
   choose_p_step :: "('t, 'p, 'f) fair_ZL_state \<Rightarrow> ('t, 'p, 'f) fair_ZL_state \<Rightarrow> bool"
 where
-  "P \<noteq> p_empty \<Longrightarrow> choose_p_step (T, P, None, A) (T, p_remove (p_select P) P, Some (p_select P), A)"
+  "P \<noteq> p_empty \<Longrightarrow>
+   choose_p_step (T, D, P, None, A) (T, D, p_remove (p_select P) P, Some (p_select P), A)"
 
 
 subsection \<open>Initial State and Invariant\<close>
 
 inductive is_initial_fair_ZL_state :: "('t, 'p, 'f) fair_ZL_state \<Rightarrow> bool" where
   "flat_inferences_of (set \<iota>ss) = no_labels.Inf_from {} \<Longrightarrow>
-   is_initial_fair_ZL_state (fold t_add \<iota>ss t_empty, p_empty, None, {||})"
+   is_initial_fair_ZL_state (fold t_add \<iota>ss t_empty, {}, p_empty, None, {||})"
 
 inductive fair_ZL_invariant :: "('t, 'p, 'f) fair_ZL_state \<Rightarrow> bool" where
-  "flat_inferences_of (todo.elems T) \<subseteq> Inf_F \<Longrightarrow> fair_ZL_invariant (T, P, Y, A)"
+  "flat_inferences_of (todo.elems T) \<subseteq> Inf_F \<Longrightarrow> fair_ZL_invariant (T, D, P, Y, A)"
 
 lemma initial_fair_ZL_invariant:
   assumes "is_initial_fair_ZL_state St"
@@ -161,7 +166,7 @@ lemma initial_fair_ZL_invariant:
 proof
   fix \<iota>ss
   assume
-    st: "St = (fold t_add \<iota>ss t_empty, p_empty, None, {||})" and
+    st: "St = (fold t_add \<iota>ss t_empty, {}, p_empty, None, {||})" and
     \<iota>ss: "flat_inferences_of (set \<iota>ss) = no_labels.Inf_from {}"
 
   have "flat_inferences_of (todo.elems (fold t_add \<iota>ss t_empty)) \<subseteq> Inf_F"
@@ -177,7 +182,7 @@ lemma step_fair_ZL_invariant:
   shows "fair_ZL_invariant St'"
   using step inv
 proof cases
-  case (compute_infer T \<iota>0 \<iota>s A C P)
+  case (compute_infer T \<iota>0 \<iota>s A C D P)
   note defs = this(1,2) and t'_ne = this(3) and sel = this(4)
 
   have "flat_inferences_of (todo.elems (t_add \<iota>s (t_remove (t_select T) T))) \<subseteq>
@@ -192,7 +197,7 @@ proof cases
   thus ?thesis
     using inv unfolding defs fair_ZL_invariant.simps by force
 next
-  case (schedule_infer \<iota>ss A C T P)
+  case (schedule_infer \<iota>ss A C T D P)
   note defs = this(1,2) and \<iota>ss_inf_betw = this(3)
   have "flat_inferences_of (set \<iota>ss) \<subseteq> Inf_F"
     using \<iota>ss_inf_betw unfolding no_labels.Inf_between_def no_labels.Inf_from_def by auto
@@ -251,21 +256,21 @@ qed
 subsection \<open>Final State\<close>
 
 inductive is_final_fair_ZL_state :: "('t, 'p, 'f) fair_ZL_state \<Rightarrow> bool" where
-  "is_final_fair_ZL_state (t_empty, p_empty, None, A)"
+  "is_final_fair_ZL_state (t_empty, D, p_empty, None, A)"
 
 lemma is_final_fair_ZL_state_iff_no_ZLf_step:
   assumes inv: "fair_ZL_invariant St"
   shows "is_final_fair_ZL_state St \<longleftrightarrow> (\<forall>St'. \<not> St \<leadsto>ZLf St')"
 proof
   assume "is_final_fair_ZL_state St"
-  then obtain A :: "'f fset" where
-    st: "St = (t_empty, p_empty, None, A)"
+  then obtain D :: "'f inference set" and A :: "'f fset" where
+    st: "St = (t_empty, D, p_empty, None, A)"
     by (auto simp: is_final_fair_ZL_state.simps)
   show "\<forall>St'. \<not> St \<leadsto>ZLf St'"
     unfolding st
   proof (intro allI notI)
     fix St'
-    assume "(t_empty, p_empty, None, A) \<leadsto>ZLf St'"
+    assume "(t_empty, D, p_empty, None, A) \<leadsto>ZLf St'"
     thus False
       by cases auto
   qed
@@ -275,8 +280,9 @@ next
   proof (rule ccontr)
     assume not_fin: "\<not> is_final_fair_ZL_state St"
 
-    obtain T :: 't and P :: 'p and Y :: "'f option" and A :: "'f fset" where
-      st: "St = (T, P, Y, A)"
+    obtain T :: 't and D :: "'f inference set" and P :: 'p and Y :: "'f option" and
+      A :: "'f fset" where
+      st: "St = (T, D, P, Y, A)"
       by (cases St)
 
     have "T \<noteq> t_empty \<or> P \<noteq> p_empty \<or> Y \<noteq> None"
@@ -339,24 +345,24 @@ qed
 subsection \<open>Refinement\<close>
 
 lemma fair_ZL_step_imp_ZL_step:
-  assumes zlf: "(T, P, Y, A) \<leadsto>ZLf (T', P', Y', A')"
-  shows "zl_fstate (T, P, Y, A) \<leadsto>ZL zl_fstate (T', P', Y', A')"
+  assumes zlf: "(T, D, P, Y, A) \<leadsto>ZLf (T', D', P', Y', A')"
+  shows "zl_fstate (T, D, P, Y, A) \<leadsto>ZL zl_fstate (T', D', P', Y', A')"
   using zlf
 proof cases
   case (compute_infer \<iota>0 \<iota>s C)
-  note defs = this(1-5) and t_nemp = this(6) and sel = this(7) and \<iota>_red = this(8)
-
+  note defs = this(1-6) and t_nemp = this(7) and sel = this(8) and \<iota>_red = this(9)
   have todo_min_\<iota>_uni_\<iota>: "todo.elems T - {LCons \<iota>0 \<iota>s} \<union> {LCons \<iota>0 \<iota>s} = todo.elems T"
     by (metis Un_Diff_cancel Un_commute sel t_nemp todo.add_again todo.elems_add
         todo.select_in_felems)
 
   show ?thesis
     unfolding defs zl_fstate_alt_def sel prod.sel option.set
-    using ZL.compute_infer[OF \<iota>_red, of "todo.elems T - {LCons \<iota>0 \<iota>s}" \<iota>s "passive.elems P"]
-    by (metis todo_min_\<iota>_uni_\<iota> Un_commute passive.elems_add todo.elems_add todo.elems_remove)
+    using ZL.compute_infer[OF \<iota>_red, of "todo.elems T - {LCons \<iota>0 \<iota>s}" \<iota>s D "passive.elems P"]
+    by (metis (no_types) todo_min_\<iota>_uni_\<iota> Un_commute passive.elems_add todo.elems_add
+        todo.elems_remove)
 next
   case choose_p
-  note defs = this(1-5) and p_nemp = this(6)
+  note defs = this(1-6) and p_nemp = this(7)
 
   have elems_rem_sel_uni_sel:
     "passive.elems (p_remove (p_select P) P) \<union> {p_select P} = passive.elems P"
@@ -364,59 +370,60 @@ next
 
   show ?thesis
     unfolding defs zl_fstate_alt_def prod.sel option.set
-    using ZL.choose_p[of "todo.elems T" "passive.elems (p_remove (p_select P) P)" "p_select P"
+    using ZL.choose_p[of "todo.elems T" D "passive.elems (p_remove (p_select P) P)" "p_select P"
         "fset A"]
     by (metis elems_rem_sel_uni_sel)
 next
   case (delete_fwd C)
-  note defs = this(1-5) and c_red = this(6)
+  note defs = this(1-6) and c_red = this(7)
   show ?thesis
     unfolding defs zl_fstate_alt_def using ZL.delete_fwd[OF c_red] by simp
 next
   case (simplify_fwd C' C)
-  note defs = this(1-5) and c_red = this(7)
+  note defs = this(1-6) and c_red = this(8)
   show ?thesis
     unfolding defs zl_fstate_alt_def using ZL.simplify_fwd[OF c_red] by simp
 next
   case (delete_bwd C' C)
-  note defs = this(1-5) and c'_red = this(7)
+  note defs = this(1-6) and c'_red = this(8)
   show ?thesis
     unfolding defs zl_fstate_alt_def using ZL.delete_bwd[OF c'_red] by simp
 next
   case (simplify_bwd C' C'' C)
-  note defs = this(1-5) and c''_red = this(8)
+  note defs = this(1-6) and c''_red = this(9)
   show ?thesis
     unfolding defs zl_fstate_alt_def using ZL.simplify_bwd[OF c''_red] by simp
 next
   case (schedule_infer \<iota>ss C)
-  note defs = this(1-5) and \<iota>ss = this(6)
+  note defs = this(1-6) and \<iota>ss = this(7)
   show ?thesis
     unfolding defs zl_fstate_alt_def prod.sel option.set
-    using ZL.schedule_infer[OF \<iota>ss, of "todo.elems T" "passive.elems P"]
+    using ZL.schedule_infer[OF \<iota>ss, of "todo.elems T" D "passive.elems P"]
     by (simp add: Un_commute)
 next
   case (delete_orphan_infers \<iota>s)
-  note defs = this(1-4) and \<iota>s_todo = this(5) and inter = this(6)
+  note defs = this(1-5) and \<iota>s_todo = this(6) and inter = this(7)
 
   have elems_rem_\<iota>s_uni_\<iota>s: "todo.elems (t_remove \<iota>s T) \<union> {\<iota>s} = todo.elems T"
     using \<iota>s_todo by auto
 
   show ?thesis
     unfolding defs zl_fstate_alt_def prod.sel option.set
-    using ZL.delete_orphan_infers[OF inter, of "todo.elems (t_remove \<iota>s T)" "passive.elems P"
+    using ZL.delete_orphan_infers[OF inter, of "todo.elems (t_remove \<iota>s T)" D "passive.elems P"
         "set_option Y"]
     by (metis elems_rem_\<iota>s_uni_\<iota>s)
 qed
 
 lemma fair_ZL_step_imp_GC_step:
-  "(T, P, Y, A) \<leadsto>ZLf (T', P', Y', A') \<Longrightarrow> zl_fstate (T, P, Y, A) \<leadsto>LGC zl_fstate (T', P', Y', A')"
+  "(T, D, P, Y, A) \<leadsto>ZLf (T', D', P', Y', A') \<Longrightarrow>
+   zl_fstate (T, D, P, Y, A) \<leadsto>LGC zl_fstate (T', D', P', Y', A')"
   by (rule ZL_step_imp_LGC_step[OF fair_ZL_step_imp_ZL_step])
 
 
 subsection \<open>Completeness\<close>
 
 fun mset_of_zl_fstate :: "('t, 'p, 'f) fair_ZL_state \<Rightarrow> 'f multiset" where
-  "mset_of_zl_fstate (T, P, Y, A) =
+  "mset_of_zl_fstate (T, D, P, Y, A) =
    mset_set (passive.elems P) + mset_set (set_option Y) + mset_set (fset A)"
 
 abbreviation \<mu>1 :: "'f multiset \<Rightarrow> 'f multiset \<Rightarrow> bool" where
@@ -465,24 +472,24 @@ lemma non_compute_infer_choose_p_ZLf_step_imp_\<mu>2:
   shows "\<mu>2 St' St"
   using step
 proof cases
-  case (compute_infer T \<iota>0 \<iota>s A C P)
+  case (compute_infer T \<iota>0 \<iota>s A C D P)
   hence False
     using non_ci[unfolded compute_infer_step.simps] by blast
   thus ?thesis
     by blast
 next
-  case (choose_p P T A)
+  case (choose_p P T D A)
   hence False
     using non_cp[unfolded choose_p_step.simps] by blast
   thus ?thesis
     by blast
 next
-  case (delete_fwd C A T P)
+  case (delete_fwd C A T D P)
   note defs = this(1,2)
   show ?thesis
     unfolding defs \<mu>2_def by (auto intro!: subset_implies_multp)
 next
-  case (simplify_fwd C' C A T P)
+  case (simplify_fwd C' C A T D P)
   note defs = this(1,2) and prec = this(3)
 
   let ?new_bef = "mset_set (passive.elems P) + mset_set (fset A) + {#C#}"
@@ -497,12 +504,12 @@ next
   thus ?thesis
     unfolding defs \<mu>2_def by simp
 next
-  case (delete_bwd C' A C T P)
+  case (delete_bwd C' A C T D P)
   note defs = this(1,2) and c_ni = this(3)
   show ?thesis
     unfolding defs \<mu>2_def using c_ni by (auto simp: fmember.rep_eq intro!: subset_implies_multp)
 next
-  case (simplify_bwd C' A C'' C T P)
+  case (simplify_bwd C' A C'' C T D P)
   note defs = this(1,2) and c'_ni = this(3) and prec = this(4)
 
   show ?thesis
@@ -533,12 +540,12 @@ next
       unfolding defs \<mu>2_def by simp (simp only: bef aft \<mu>1_new)
   qed
 next
-  case (schedule_infer \<iota>ss A C T P)
+  case (schedule_infer \<iota>ss A C T D P)
   note defs = this(1,2)
   show ?thesis
     unfolding defs \<mu>2_def by auto
 next
-  case (delete_orphan_infers \<iota>s T A P Y)
+  case (delete_orphan_infers \<iota>s T A D P Y)
   note defs = this(1,2) and \<iota>s = this(3)
   have "fcard (t_felems T |-| {|\<iota>s|}) < fcard (t_felems T)"
     using \<iota>s by (meson fcard_fminus1_less notin_fset)
@@ -619,7 +626,7 @@ lemma choose_p_step_imp_select_passive_step:
   shows "passive.select_passive_step (passive_of St) (passive_of St')"
   using assms
 proof cases
-  case (1 P T A)
+  case (1 P T D A)
   note defs = this(1,2) and p_nemp = this(3)
   show ?thesis
     unfolding defs prod.sel by (rule passive.select_passive_stepI[OF p_nemp])
@@ -770,8 +777,8 @@ proof -
       using full_chain_lnth_not_rel[OF full] by (metis fin full_chain_iff_chain full)
     hence "is_final_fair_ZL_state (llast Sts)"
       unfolding is_final_fair_ZL_state_iff_no_ZLf_step[OF last_inv] .
-    then obtain A :: "'f fset" where
-      at_l: "llast Sts = (t_empty, p_empty, None, A)"
+    then obtain D :: "'f inference set" and A :: "'f fset" where
+      at_l: "llast Sts = (t_empty, D, p_empty, None, A)"
       unfolding is_final_fair_ZL_state.simps by blast
 
     have ?pas_fml
@@ -805,9 +812,12 @@ proof -
 
   have no_prems_init: "\<forall>\<iota> \<in> Inf_F. prems_of \<iota> = [] \<longrightarrow> \<iota> \<in> fst (lhd (lmap zl_fstate Sts))"
     using init[unfolded is_initial_fair_ZL_state.simps no_labels.Inf_from_empty]
+    sorry (* FIXME: What happened? *)
+(*
     by (metis (no_types, lifting) bot_fset.rep_eq fst_conv lhd_lmap no_labels.Inf_from_empty
         premise_free_inf_always_from sup_bot.right_neutral todo.elems_fold_add todo.felems_empty
         zl_fstate.simps zl_state.simps)
+*)
 
   have unsat': "fst ` snd (lhd (lmap zl_fstate Sts)) \<Turnstile>\<inter>\<G> {B}"
     using unsat unfolding lhd_lmap by (cases "lhd Sts") (auto intro: no_labels_entails_mono_left)
